src/ReactorModel/Execution/Schedule.lean
@@ -6,15 +6,16 @@ namespace Execution
 --       If we schedule something for the past, it doesn't matter, since that action value will never be read.
 --       But if the current tag has a microstep of 0, it is possible to schedule something for the current tag
 --       (in the `none` case).
-noncomputable def schedule (act : Time.Tag ⇉ Value) (t : Time) (v : Value) : Time.Tag ⇉ Value :=
-  match act.ids.filter (·.time = t) |>.max with
-  | none => act.update ⟨t, 0⟩ v
-  | some g => act.update ⟨t, g.microstep + 1⟩ v
+def schedule (act : Time.Tag ⇉ Value) (t : Time) (v : Value) : Time.Tag ⇉ Value :=
+  match act.keys.filter (·.time = t) |>.max with
+  | ⊥ => act.insert ⟨t, 0⟩ v
+  | some ⟨_, m⟩ => act.insert ⟨t, m + 1⟩ v
 
-theorem schedule_preserves_unchanged_time (h : t ≠ t') : a ⟨t', m⟩ = schedule a t v ⟨t', m⟩ := by
+theorem schedule_preserves_unchanged_time (h : t ≠ t') : 
+    a ⟨t', m⟩ = schedule a t v ⟨t', m⟩ := by
   sorry
 
-noncomputable def schedule' (act : Time.Tag ⇉ Value) (t : Time) : (List Value) → Time.Tag ⇉ Value
+def schedule' (act : Time.Tag ⇉ Value) (t : Time) : (List Value) → Time.Tag ⇉ Value
   | .nil => act
   | .cons v tl => schedule' (schedule act t v) t tl
 
@@ -22,8 +23,9 @@ theorem schedule'_cons (act : Time.Tag ⇉ Value) :
     schedule' act t (hd :: tl) = schedule' (schedule act t hd) t tl := 
   rfl
 
-theorem schedule'_tag_congr {act₁ act₂ : Time.Tag ⇉ Value} (h : act₁ ⟨t, m⟩ = act₂ ⟨t, m⟩) :
-    (schedule' act₁ t l) ⟨t, m⟩ = (schedule' act₂ t l) ⟨t, m⟩ :=
+theorem schedule'_tag_congr {act₁ act₂ : Time.Tag ⇉ Value} 
+    (h : act₁ ⟨t, m⟩ = act₂ ⟨t, m⟩) :
+    schedule' act₁ t l ⟨t, m⟩ = schedule' act₂ t l ⟨t, m⟩ :=
   sorry
 
 end Execution
