src/ReactorModel/Extensions.lean
@@ -1,5 +1,6 @@
 import Mathlib.Data.Finset.Basic
 import Mathlib.Data.Set.Finite
+import Mathlib.Data.Finmap
 import Mathlib.Tactic.LibrarySearch
 
 open Lean
@@ -52,12 +53,8 @@ theorem lastSome?_tail :
 
 end List
 
-namespace Finset 
-
-theorem ssubset_ne {s₁ s₂ : Finset α} (h : s₁ ⊂ s₂) : s₁ ≠ s₂ := 
+theorem Set.ssubset_ne {s₁ s₂ : Set α} (h : s₁ ⊂ s₂) : s₁ ≠ s₂ :=
   ssubset_iff_subset_ne.mp h |>.right
-
-end Finset
 
 abbrev Partial (α β) := α → Option β
 
@@ -95,174 +92,19 @@ theorem map_inj {f₁ f₂ : α ⇀ β} (hi : g.Injective) (h : f₁.map g = f�
 theorem attach_map_val (f : α ⇀ β) : f.attach.map Subtype.val = f := by
   sorry
 
--- TODO: Is this used anywhere?
-def filter (f : α ⇀ β) (p : β → Prop) [DecidablePred p] : α ⇀ β := 
-  fun a => f a >>= fun b => if p b then b else none
+def restrict (f : α ⇀ β) (s : Set α) [DecidablePred (· ∈ s)] : α ⇀ β := 
+  fun a => if a ∈ s then f a else none 
+
+def filterMap (f : α ⇀ β) (g : β → Option γ) : α ⇀ γ := 
+  fun a => f a >>= g
 
 end Partial
 
-
--- TODO: Remove Finmap?
-
--- We need to use our own `Finmap` type based on `α → Option β`, as this is integral for the 
--- definition of `RawReactor`.
-structure Finmap (α β) where
-  lookup : α → Option β 
-  finite : { a | lookup a ≠ none }.Finite
-
 namespace Finmap
 
-variables {α β : Type _} [DecidableEq α] [DecidableEq β]  
+infixr:50 " ⇉ " => (Finmap fun _ : · => ·)
 
-infixr:50 " ⇉ " => Finmap
-
--- A coercion so that finmaps can be called directly as functions.
-instance : CoeFun (α ⇉ β) (fun _ => α → Option β) where
+instance [DecidableEq α] : CoeFun (α ⇉ β) (fun _ => α → Option β) where
   coe f := f.lookup
-
--- This allows us to use `∅` as notation for the empty finite map.
-instance : EmptyCollection (α ⇉ β) where 
-  emptyCollection := { lookup := (fun _ => none), finite := by simp }  
-
-instance : Inhabited (Finmap α β) where
-  default := ∅
-
-@[ext]
-theorem ext : {f₁ f₂ : α ⇉ β} → (h : ∀ a, f₁ a = f₂ a) → f₁ = f₂
-  | mk .., mk .., h => by simp; funext a; exact h a
-
--- The (finite) set of inputs for which a given finmap has an associated value.
-noncomputable def ids (f : α ⇉ β) : Finset α :=
-  f.finite.toFinset
-
-theorem mem_ids_iff {f : α ⇉ β} : i ∈ f.ids ↔ ∃ b, f i = some b := by
-  sorry
-
--- The (finite) set of values for which there exist inputs that map to them.
-noncomputable def values (f : α ⇉ β) : Finset β :=
-  let description := { v : β | ∃ i, f i = v }
-  let finite : description.Finite := by
-    let s := f.ids.image f.lookup
-    let t := { v | ∃ i, f i = some v }.image Option.some
-    suffices h : t ⊆ ↑s from sorry -- Set.Finite.subset (Finset.finite_toSet s) h
-    intro x h
-    simp at *
-    have ⟨b, ⟨a, ha⟩, hb⟩ := h
-    exists a
-    apply And.intro
-    case left => sorry -- simp [ids_def, ha]
-    case right => simp [ha, hb]
-  finite.toFinset
- 
-theorem mem_values_iff {f : α ⇉ β} : v ∈ f.values ↔ (∃ i, f i = some v) := by
-  simp [values, Set.Finite.mem_toFinset, Set.mem_setOf_eq]
-
-def update (f : α ⇉ β) (a : α) (b : β) : α ⇉ β := {
-  lookup := Function.update f.lookup a b,
-  finite := sorry
-}
-
-theorem update_self (f : α ⇉ β) (a : α) (b : β) : (f.update a b) a = b :=
-  sorry
-
-theorem update_ne (f : α ⇉ β) (h : a ≠ a') (b : β) : (f.update a b) a' = f a' :=
-  sorry
-
-def map (f : α ⇉ β) (g : β → γ) : α ⇉ γ := {
-  lookup := fun a => (f a) >>= (some ∘ g),
-  finite := by
-    suffices h : { a | (fun i => (f i) >>= (some ∘ g)) a ≠ none } ⊆ ↑f.ids
-      from Set.Finite.subset (Finset.finite_toSet _) h
-    intro x h
-    sorry
-}
-
-theorem map_mem_ids {f : α ⇉ β} : i ∈ (f.map g).ids ↔ i ∈ f.ids :=
-  sorry
-
-theorem map_def {f : α ⇉ β} (h : (f.map g) i = some v) : ∃ m, f i = some m ∧ g m = v :=
-  sorry
-
-noncomputable def map' (f : α ⇉ γ) (g : α → Option β) (h : g.Injective) : β ⇉ γ := {
-  lookup := fun b => 
-    if h : ∃ a ∈ f.ids, g a = b -- This is unique because of h.
-    then f h.choose
-    else none
-  finite := sorry
-}
-
-theorem map'_def {f : α ⇉ γ} {g : α → Option β} {h} : (g a = some b) → (f.map' g h b = f a) :=
-  sorry   
-
-def attach (f : α ⇉ β) : α ⇉ { b // b ∈ f.values } := {
-  lookup := fun a =>
-    match h:(f a) with
-    | none => none
-    | some b => some ⟨b, (mem_values_iff.mpr ⟨a, h⟩)⟩,
-  finite := sorry
-}
-
-theorem attach_mem_ids {f : α ⇉ β} {i} : i ∈ f.attach.ids ↔ i ∈ f.ids :=
-  sorry
-
-theorem attach_def {f : α ⇉ β} {i} {b : β} {hb} (h : f.attach i = some ⟨b, hb⟩) : f i = b :=
-  sorry
-
--- The finmap that contains only those entries from `f`, whose identifiers
--- satisfy the given predicate `p`.
-noncomputable def filter (f : α ⇉ β) (p : α → Prop) [DecidablePred p] : α ⇉ β := {
-  lookup := fun a => if p a then f a else none,
-  finite := sorry
-}
-
--- The finmap that contains only those entries from `f`, whose values
--- satisfy the given predicate `p`.
-noncomputable def filter' (f : α ⇉ β) (p : β → Prop) [DecidablePred p] : α ⇉ β := {
-  lookup := (fun a => 
-    match f a with
-    | some b => if p b then b else none
-    | none => none
-  ),
-  finite := sorry
-}
-
-variable {p : β → Prop} [DecidablePred p]
-
-theorem filter'_mem {f : α ⇉ β} {i : α} {b : β} : 
-  (f.filter' p) i = some b ↔ f i = b ∧ p b :=
-  sorry
-
-theorem filter'_mem_values {f : α ⇉ β} {b : β} : 
-  b ∈ (f.filter' p).values ↔ ∃ i : α, f i = b ∧ p b :=
-  sorry 
-
-def filterMap (f : α ⇉ β) (g : β → Option γ) : α ⇉ γ := {
-  lookup := fun a => (f a) >>= g,
-  finite := sorry
-}
-
-theorem filterMap_congr {f₁ f₂ : α ⇉ β} : (f₁ a = f₂ a) → (f₁.filterMap g a = f₂.filterMap g a) :=
-  sorry
-
--- The finmap that containts only those entries from `f`, whose identifiers
--- are in a given set `as`.
-noncomputable def restrict (f : α ⇉ β) (as : Finset α) : α ⇉ β :=
-  f.filter (fun a => a ∈ as)
-
-theorem restrict_ext {f₁ f₂ : α ⇉ β} {as : Finset α} : 
-  (∀ a ∈ as, f₁ a = f₂ a) → f₁.restrict as = f₂.restrict as := 
-  sorry
-
-structure Forall₂ (r : β → γ → Prop) (f₁ : α ⇉ β) (f₂ : α → Option γ) : Prop where
-  eqIDs : ∀ a, a ∈ f₁.ids ↔ f₂ a ≠ none
-  rel : ∀ {a} {b : β} {c : γ}, (f₁ a = b) → (f₂ a = c) → r b c
-
-def union (f₁ f₂ : α ⇉ β) : α ⇉ β := {
-  lookup := fun a => (f₁ a).elim (f₂ a) .some,
-  finite := sorry
-}
-
-instance : Union (α ⇉ β) where 
-  union := union
 
 end Finmap
