src/ReactorModel/Determinism/ChangeStep.lean
@@ -12,54 +12,54 @@ theorem preserves_tag (e : s₁ -[c]→ s₂) : s₁.tag = s₂.tag := by
   cases e <;> rfl
 
 theorem preserves_rcns {i : ID} (e : s₁ -[c]→ s₂) : s₁.rtr[.rcn][i] = s₂.rtr[.rcn][i] := by
-  cases e <;> first | rfl | simp [Reactor.Update.preserves_ne_cmp_or_id ‹_›]
+  sorry
 
 theorem equiv (e : s₁ -[c]→ s₂) : s₁.rtr ≈ s₂.rtr := by
   cases e 
   case' port h, state h, action h => exact h.equiv
   all_goals exact .refl 
 
-theorem preserves_unchanged_port (e : s₁ -[c]→ s₂) (h : ¬c.obj.IsPort i := by exact (nomatch ·)) :
+theorem preserves_unchanged_port (e : s₁ -[c]→ s₂) (h : ¬c.obj.IsPortᵢ i := by exact (nomatch ·)) :
     s₁.rtr[.prt][i] = s₂.rtr[.prt][i] := by
   cases e
-  case port u => simp [Change.IsPort.iff_id_eq] at h; exact u.preserves_ne_id h
+  case port u => simp [Change.IsPortᵢ.iff_id_eq] at h; exact u.preserves_ne_id h
   case' state u, action u => exact u.preserves_ne_cmp
   all_goals rfl
 
-theorem preserves_unchanged_state (e : s₁ -[c]→ s₂) (h : ¬c.obj.IsState i := by exact (nomatch ·)) : 
+theorem preserves_unchanged_state (e : s₁ -[c]→ s₂) (h : ¬c.obj.IsStateᵢ i := by exact (nomatch ·)) : 
     s₁.rtr[.stv][i] = s₂.rtr[.stv][i] := by
   cases e
-  case state u => simp [Change.IsState.iff_id_eq] at h; exact u.preserves_ne_id h
+  case state u => simp [Change.IsStateᵢ.iff_id_eq] at h; exact u.preserves_ne_id h
   case' action u, port u => exact u.preserves_ne_cmp
   all_goals rfl
 
 theorem preserves_unchanged_action 
-    (e : s₁ -[c]→ s₂) (h : ¬c.obj.IsAction i := by exact (nomatch ·)) : 
+    (e : s₁ -[c]→ s₂) (h : ¬c.obj.IsActionᵢ i := by exact (nomatch ·)) : 
     s₁.rtr[.act][i] = s₂.rtr[.act][i] := by
   cases e 
-  case action u => simp [Change.IsAction.iff_id_eq] at h; exact u.preserves_ne_id h
+  case action u => simp [Change.IsActionᵢ.iff_id_eq] at h; exact u.preserves_ne_id h
   case' state u, port u => exact u.preserves_ne_cmp 
   all_goals rfl
 
 theorem port_change : 
     (s₁ -[⟨rcn, .port i v⟩]→ s₂) → ∃ k, s₂.rtr[.prt][i] = some { val := v, kind := k }
   | port u => by
-    have ⟨p, _, _⟩ := u.change'
+    have ⟨p, _, _⟩ := u.change
     exists p.kind    
 
 theorem state_change : (s₁ -[⟨rcn, .state i v⟩]→ s₂) → s₂.rtr[.stv][i] = some v
-  | state u => u.change'.choose_spec.right
+  | state u => u.change.choose_spec.right
 
 theorem action_change {i : ID} (h : s₁.rtr[.act][i] = some a) :
     (s₁ -[⟨rcn, .action i t v⟩]→ s₂) → s₂.rtr[.act][i] = some (schedule a t v)
   | action u => by
-    have ⟨_, h₁, h₂⟩ := u.change'
+    have ⟨_, h₁, h₂⟩ := u.change
     simp_all [h, h₁, h₂]
 
 theorem port_change' {i : ID} (h : s₁.rtr[.prt][i] = some p) :
     (s₁ -[⟨rcn, .port i v⟩]→ s₂) → s₂.rtr[.prt][i] = some { p with val := v }
   | port u => by
-    have ⟨_, h₁, h₂⟩ := u.change'
+    have ⟨_, h₁, h₂⟩ := u.change
     simp_all [h, h₁, h₂]
 
 theorem port_preserves_port_kind {j : ID} 
@@ -67,12 +67,12 @@ theorem port_preserves_port_kind {j : ID}
     ∃ v, s₂.rtr[.prt][j] = some { p with val := v } :=
   if hi : i = j
   then ⟨v, hi ▸ e.port_change' (hi ▸ h)⟩ 
-  else ⟨_, e.preserves_unchanged_port (Change.IsPort.iff_id_eq.not.mpr hi) ▸ h⟩ 
+  else ⟨_, e.preserves_unchanged_port (Change.IsPortᵢ.iff_id_eq.not.mpr hi) ▸ h⟩ 
 
 theorem preserves_port_kind {i : ID} (e : s₁ -[⟨rcn, c⟩]→ s₂) (h : s₁.rtr[.prt][i] = some p) :
     ∃ v, s₂.rtr[.prt][i] = some { p with val := v } := by
-  cases c
-  case port => exact e.port_preserves_port_kind h
+  cases c <;> try cases ‹Change.Normal›   
+  case norm.port => exact e.port_preserves_port_kind h
   all_goals
     simp [←e.preserves_unchanged_port (i := i), h]
     exists p.val
@@ -92,7 +92,7 @@ theorem action_preserves_action_at_unchanged_times
     a₁ ⟨t', m⟩ = a₂ ⟨t', m⟩ := by
   by_cases hi : i = j
   case neg =>
-    have h := e.preserves_unchanged_action (i := j) (Change.IsAction.iff_id_eq.not.mpr hi) 
+    have h := e.preserves_unchanged_action (i := j) (Change.IsActionᵢ.iff_id_eq.not.mpr hi) 
     simp_all [ho₁, ho₂, h]
   case pos =>
     have ht := hc.resolve_left (not_not.mpr hi)
@@ -100,12 +100,12 @@ theorem action_preserves_action_at_unchanged_times
 
 -- Note: `ho₁` and `e` imply that there exists some `a₂` such that `ho₂`.
 theorem preserves_action_at_unchanged_times
-    (e : s₁ -[⟨rcn, c⟩]→ s₂) (hc : ¬c.IsActionAt i t) 
+    (e : s₁ -[⟨rcn, c⟩]→ s₂) (hc : ¬c.IsActionₜ i t) 
     (ho₁ : s₁.rtr[.act][i] = some a₁) (ho₂ : s₂.rtr[.act][i] = some a₂) :
     a₁ ⟨t, m⟩ = a₂ ⟨t, m⟩ := by
-  cases c
-  case action j t v =>
-    have ht := Change.not_IsActionAt_ne_ids_or_ne_time hc
+  cases c <;> try cases ‹Change.Normal›   
+  case norm.action j t v =>
+    have ht := Change.IsActionₜ.not_to_ne_ids_or_ne_time hc
     exact e.action_preserves_action_at_unchanged_times ht ho₁ ho₂
   all_goals
     injection ho₁ ▸ ho₂ ▸ e.preserves_unchanged_action with h
@@ -113,9 +113,9 @@ theorem preserves_action_at_unchanged_times
 
 -- This theorem upgrades `preserves_action_at_unchanged_times`.
 theorem preserves_action_at_unchanged_times'
-    (e : s₁ -[⟨rcn, c⟩]→ s₂) (hc : ¬c.IsActionAt i t) (ho₁ : s₁.rtr[.act][i] = some a₁) :
+    (e : s₁ -[⟨rcn, c⟩]→ s₂) (hc : ¬c.IsActionₜ i t) (ho₁ : s₁.rtr[.act][i] = some a₁) :
     ∃ a₂, (s₂.rtr[.act][i] = some a₂) ∧ (a₁ ⟨t, m⟩ = a₂ ⟨t, m⟩) := by
-  have ⟨a₂, ho₂⟩ := e.equiv.obj?_iff.mp ⟨_, ho₁⟩ 
+  have ⟨a₂, ho₂⟩ := e.equiv.obj?_some_iff.mp ⟨_, ho₁⟩ 
   exists a₂, ho₂
   exact e.preserves_action_at_unchanged_times hc ho₁ ho₂
 
@@ -127,7 +127,7 @@ theorem context_agnostic (e : s₁ -[c]→ s) (h : s₁.rtr = s₂.rtr) :
     constructor <;> assumption
 
 theorem deterministic (e₁ : s -[c]→ s₁) (e₂ : s -[c]→ s₂) : s₁ = s₂ := by
-  cases e₁ <;> cases e₂ <;> simp <;> try apply Reactor.Update.unique' ‹_› ‹_› 
+  cases e₁ <;> cases e₂ <;> simp <;> try apply Reactor.Update.unique ‹_› ‹_› 
 
 end ChangeStep
 end Execution
