src/ReactorModel/Determinism/Execution.lean
@@ -23,7 +23,7 @@ theorem nontrivial_deterministic [State.Nontrivial s] :
     nontrivial_deterministic (e₁.deterministic e₂ ▸ e₁') e₂' ht hp
   | refl, step e e', ht, hp | step e e', refl, ht, hp => 
     match seq_progress_ssubset_or_tag_lt e e' with
-    | .inl h => absurd hp $ Finset.ssubset_ne (by simp_all) 
+    | .inl h => absurd hp $ Set.ssubset_ne (by simp_all) 
     | .inr h => absurd ht $ ne_of_lt (by simp_all)
 
 theorem deterministic : 
