src/ReactorModel/Objects/Reactor/ReactorType/Indexable.lean
@@ -54,8 +54,8 @@ noncomputable def obj? [ind : ReactorType.Indexable α] (rtr : α) :
   | .rtr, .nest i => rtr[.rtr][i]& >>= (cmp? .rtr ·.obj i)
   | .rtr, ⊤       => rtr
 
+notation rtr "[" cmp "]" => ReactorType.Indexable.obj? rtr cmp
 notation rtr "[" cmp "][" i "]" => ReactorType.Indexable.obj? rtr cmp i
-
 variable [a : Indexable α]
 
 theorem con?_eq_some {rtr : α} {cmp} (h : rtr[cmp][i]& = some con) : 
